theories/simulations/msim/MSim.v
@@ -5,39 +5,66 @@ Require Import Sandbox Mod LSim MSimCommon.
 
 Section msim.
   Context {Σ : GRA}.
-  Variable contextual: contextuality.
-  Variable fl_src : alist (option string) (Any.t → itree crisE Any.t).
-  Variable fl_tgt : alist (option string) (Any.t → itree crisE Any.t).
-  Variable Ist : ist_type Σ.
+  Context (ctx : contextuality).
+  Context (fl_src fl_tgt : gmap (option string) (option (Any.t → itree crisE Any.t))).
+  Context (Ist : ist_type Σ).
 
+  (** hsupd properties **)
   (* Note : iProp-style definition of hsupd (λ fmr, Own fmr ⊢ ∃ fmr0, |==> ⌜P fmr0⌝)
       incurs positivity problem when defining _msim. *)
   Definition hsupd (P : Σ → Prop) : Σ → Prop :=
     λ fmr, ✓ fmr → ∃ fmr0, P fmr0 ∧ (Own fmr ⊢ |==> Own fmr0).
+
+  Lemma hsupd_mon P Q r (IN : hsupd P r) (LE : P <1= Q) : hsupd Q r.
+  Proof using. by intros wf; specialize (IN wf); inv IN; exists x; split; des; eauto. Qed.
+  Lemma hsupd_incl P : P <1= hsupd P.
+  Proof using. ii; esplits; eauto. Qed.
+
+  Lemma hsupd_merge P r (REL : hsupd (hsupd P) r) : hsupd P r.
+  Proof using.
+    intros wf; specialize (REL wf); destruct REL as [r1 [??]].
+    hexploit Own_wand_valid; eauto.
+    intros wf1; hexploit (H wf1); intros [fmr0 [??]]; exists fmr0; esplits; eauto.
+    iIntros "R"; iPoseProof (H0 with "R") as "> R1"; iApply H2; done.
+  Qed.
+
+  Lemma hsupd_update P r r' (IN : hsupd P r) (UPD : r' ~~> r) :
+    hsupd P r'.
+  Proof using.
+    dup UPD; rewrite cmra_discrete_update in UPD; specialize (UPD (Some ε)); ss; rewrite ?right_id in UPD.
+    intros wfr'; hexploit (IN (UPD wfr')); i; des; eexists; split; eauto.
+    iIntros "H"; iPoseProof (Own_Upd with "H") as "> H"; first eauto.
+    iApply H0; done.
+  Qed.
+
+  Lemma hsupd_extends P r r' (IN : hsupd P r) (UPD : r ≼ r') :
+    hsupd P r'.
+  Proof using. eapply hsupd_update; eauto; eapply cmra_update_included; eauto. Qed.
+
+  Lemma hsupd_wf P r (IN : ✓ r → hsupd P r) :
+    hsupd P r.
+  Proof using. intros wf; hexploit (IN wf wf); i; des; clarify; esplits; eauto. Qed.
 
   Variant _msim'
       (msimc : ∀ Rs Rt (RR : retr_type Σ Rs Rt), msim_type Σ Rs Rt)
       {Rs Rt} {RR : retr_type Σ Rs Rt}
       (msimi : msim_type Σ Rs Rt) : msim_type Σ Rs Rt :=
 
-  | msim_ret
-      (MSIM_RET : True)
+  | msim_ret (MSIM_RET : True)
       ps pt st_src st_tgt fmr
       v_src v_tgt
       (RET : Own fmr ⊢ |==> RR (st_src, v_src) (st_tgt, v_tgt)) :
     _msim' msimc msimi ps pt (st_src, Ret v_src) (st_tgt, Ret v_tgt) fmr
 
-  | msim_call
-      (MSIM_CALL : True)
+  | msim_call (MSIM_CALL : True)
       ps pt st_src st_tgt fmr
       fn varg k_src k_tgt FR
       (INV : Own fmr ⊢ |==> (Ist st_src st_tgt ∗ FR))
       (K : ∀ vret st_src0 st_tgt0 fmr0
-            (NODS : List.NoDup (List.map fst st_src0))
-            (NODT : List.NoDup (List.map fst st_tgt0))
+            (* (NODS : List.NoDup (List.map fst st_src0))
+            (NODT : List.NoDup (List.map fst st_tgt0)) *)
             (INV : Own fmr0 ⊢ |==> (Ist st_src0 st_tgt0 ∗ FR)),
-        msimi true true (st_src0, k_src vret) (st_tgt0, k_tgt vret) fmr0)
-    :
+        msimi true true (st_src0, k_src vret) (st_tgt0, k_tgt vret) fmr0) :
     _msim' msimc msimi ps pt
       (st_src, trigger (Call fn varg) >>= k_src) (st_tgt, trigger (Call fn varg) >>= k_tgt) fmr
 
@@ -45,8 +72,7 @@ Section msim.
       (MSIM_IO : True)
       ps pt st_src st_tgt fmr
       I O fn (varg : I) k_src k_tgt
-      (K : ∀ (vret : O), msimi true true (st_src, k_src vret) (st_tgt, k_tgt vret) fmr)
-    :
+      (K : ∀ (vret : O), msimi true true (st_src, k_src vret) (st_tgt, k_tgt vret) fmr) :
     _msim' msimc msimi ps pt
       (st_src, trigger (IO fn varg) >>= k_src) (st_tgt, trigger (IO fn varg) >>= k_tgt) fmr
 
@@ -54,18 +80,16 @@ Section msim.
       (MSIM_INLINE_SRC : True)
       ps pt st_src st_tgt fmr
       fn f varg k_src i_tgt
-      (FUN : alist_find (Some fn) fl_src = Some f)
-      (K : msimi true pt (st_src, f varg >>= (λ ret, tau;; Ret ret) >>= k_src) (st_tgt, i_tgt) fmr)
-    :
+      (FUN : fl_src !! (Some fn) = Some (Some f))
+      (K : msimi true pt (st_src, f varg >>= (λ ret, tau;; Ret ret) >>= k_src) (st_tgt, i_tgt) fmr) :
     _msim' msimc msimi ps pt (st_src, trigger (Call fn varg) >>= k_src) (st_tgt, i_tgt) fmr
 
   | msim_inline_tgt
       (MSIM_INLINE_TGT : True)
       ps pt st_src st_tgt fmr
       fn f varg i_src k_tgt
-      (FUN : alist_find (Some fn) fl_tgt = Some f)
-      (K : msimi ps true (st_src, i_src) (st_tgt, f varg >>= (λ ret, tau;; Ret ret) >>= k_tgt) fmr)
-    :
+      (FUN : fl_tgt !! (Some fn) = Some (Some f))
+      (K : msimi ps true (st_src, i_src) (st_tgt, f varg >>= (λ ret, tau;; Ret ret) >>= k_tgt) fmr) :
     _msim' msimc msimi ps pt (st_src, i_src) (st_tgt, trigger (Call fn varg) >>= k_tgt) fmr
 
   | msim_tau_src
@@ -121,7 +145,7 @@ Section msim.
       ps pt st_src st_src0 st_tgt fmr
       k_src i_tgt
       k v
-      (run : st_src0 = alist_upd k v st_src)
+      (run : st_src0 = <[k := Some v]> st_src)
       (K : msimi true pt (st_src0, k_src tt) (st_tgt, i_tgt) fmr)
     :
     _msim' msimc msimi ps pt (st_src, trigger (SPut k v) >>= k_src) (st_tgt, i_tgt) fmr
@@ -131,7 +155,7 @@ Section msim.
       ps pt st_src st_tgt st_tgt0 fmr
       i_src k_tgt
       k v
-      (run : st_tgt0 = alist_upd k v st_tgt)
+      (run : st_tgt0 = <[k := Some v]> st_tgt)
       (K : msimi ps true (st_src, i_src) (st_tgt0, k_tgt tt) fmr)
     :
     _msim' msimc msimi ps pt (st_src, i_src) (st_tgt, trigger (SPut k v) >>= k_tgt) fmr
@@ -141,7 +165,7 @@ Section msim.
       ps pt st_src st_tgt fmr
       k_src i_tgt
       k v
-      (run : v = or_else (alist_find k st_src) tt↑)
+      (run : v = default tt↑ (mjoin (st_src !! k)))
       (K : msimi true pt (st_src, k_src v) (st_tgt, i_tgt) fmr)
     :
     _msim' msimc msimi ps pt (st_src, trigger (SGet k) >>= k_src) (st_tgt, i_tgt) fmr
@@ -151,7 +175,7 @@ Section msim.
       ps pt st_src st_tgt fmr
       i_src k_tgt
       k v
-      (run : v = or_else (alist_find k st_tgt) tt↑)
+      (run : v = default tt↑ (mjoin (st_tgt !! k)))
       (K : msimi ps true (st_src, i_src) (st_tgt, k_tgt v) fmr)
     :
     _msim' msimc msimi ps pt (st_src, i_src) (st_tgt, trigger (SGet k) >>= k_tgt) fmr
@@ -231,8 +255,8 @@ Section msim.
       tid k_src k_tgt FR
       (INV : Own fmr ⊢ |==> (Ist st_src st_tgt ∗ FR))
       (K : ∀ st_src0 st_tgt0 fmr0
-          (NODS : List.NoDup (List.map fst st_src0))
-          (NODT : List.NoDup (List.map fst st_tgt0))
+          (* (NODS : List.NoDup (List.map fst st_src0))
+          (NODT : List.NoDup (List.map fst st_tgt0)) *)
           (INV : Own fmr0 ⊢ |==> (Ist st_src0 st_tgt0 ∗ FR)),
         msimi true true (st_src0, k_src ()) (st_tgt0, k_tgt ()) fmr0)
     :
@@ -251,8 +275,8 @@ Section msim.
       (MSIM_CALL_NONE: True)
       ps pt st_src st_tgt fmr
       fn varg k_src i_tgt
-      (CLOSED: contextual = closed)
-      (FUN: alist_find (Some fn) fl_src = None)
+      (CLOSED: ctx = closed)
+      (FUN: mjoin (fl_src !! (Some fn)) = None)
     :
     _msim' msimc msimi ps pt (st_src, trigger (Call fn varg) >>= k_src) (st_tgt, i_tgt) fmr
 
@@ -260,8 +284,8 @@ Section msim.
       (MSIM_SPAWN_NONE: True)
       ps pt st_src st_tgt fmr
       fn varg k_src i_tgt
-      (CLOSED: contextual = closed)
-      (FUN: alist_find (Some fn) fl_src = None)
+      (CLOSED: ctx = closed)
+      (FUN: mjoin (fl_src !! (Some fn)) = None)
     :
     _msim' msimc msimi ps pt (st_src, trigger (Spawn fn varg) >>= k_src) (st_tgt, i_tgt) fmr
 
@@ -271,27 +295,25 @@ Section msim.
       (SIM : msimc Rs Rt RR false false sti_src sti_tgt fmr)
     :
     _msim' msimc msimi true true sti_src sti_tgt fmr.
-
   Global Arguments _msim' msimc {Rs Rt} RR msimi.
 
   Inductive _msim msim Rs Rt RR ps pt sti_src sti_tgt fmr : Prop :=
   | msim_intro
-      (IN :
-        ∀ (NODFS : List.NoDup (List.map fst fl_src))
-          (NODFT : List.NoDup (List.map fst fl_tgt))
-          (NODS : List.NoDup (List.map fst sti_src.1))
-          (NODT : List.NoDup (List.map fst sti_tgt.1)),
+      (IN : ∀ (NODFS : map_Forall (const is_Some) (fl_src))
+               (NODFT : map_Forall (const is_Some) (fl_tgt))
+               (NODS : map_Forall (const is_Some) (sti_src.1))
+               (NODT : map_Forall (const is_Some) (sti_tgt.1)),
         hsupd (@_msim' msim Rs Rt RR (@_msim msim Rs Rt RR) ps pt sti_src sti_tgt) fmr).
 
   Definition msim {Rs Rt} RR := paco8 _msim bot8 Rs Rt RR.
 
   Lemma _msim_tarski msim Rs Rt RR rel
       (FIX : ∀ ps pt sti_src sti_tgt fmr
-             (IN : ∀ (NODFS : List.NoDup (List.map fst fl_src))
-                     (NODFT : List.NoDup (List.map fst fl_tgt))
-                     (NODS : List.NoDup (List.map fst sti_src.1))
-                     (NODT : List.NoDup (List.map fst sti_tgt.1)),
-              hsupd (@_msim' msim Rs Rt RR rel ps pt sti_src sti_tgt) fmr),
+             (IN : ∀ (NODFS : map_Forall (const is_Some) (fl_src))
+                (NODFT : map_Forall (const is_Some) (fl_tgt))
+                (NODS : map_Forall (const is_Some) (sti_src.1))
+                (NODT : map_Forall (const is_Some) (sti_tgt.1)),
+                hsupd (@_msim' msim Rs Rt RR rel ps pt sti_src sti_tgt) fmr),
         rel ps pt sti_src sti_tgt fmr) :
     _msim msim Rs Rt RR <5= rel.
   Proof using.
@@ -304,9 +326,6 @@ Section msim.
       eauto using @_msim' with paco.
   Qed.
 
-  Lemma hsupd_mon P Q r (IN : hsupd P r) (LE : P <1= Q) : hsupd Q r.
-  Proof using. by intros wf; specialize (IN wf); inv IN; exists x; split; des; eauto. Qed.
-
   Lemma _msim'_mon r r' Rs Rt RR s s'
       ps pt sti_src sti_tgt fmr
       (REL : @_msim' r Rs Rt RR s ps pt sti_src sti_tgt fmr)
@@ -318,10 +337,7 @@ Section msim.
   Qed.
 
   Lemma _msim_mon : monotone8 _msim.
-  Proof using.
-    ii. eapply _msim_tarski, IN.
-    i. econs. eauto using hsupd_mon, _msim'_mon.
-  Qed.
+  Proof using. ii. eapply _msim_tarski, IN. i. econs. eauto using hsupd_mon, _msim'_mon. Qed.
 
   Lemma _msim_mon_auto r r' Rs Rt RR
       ps pt sti_src sti_tgt fmr
@@ -336,36 +352,8 @@ Section msim.
   Hint Resolve hsupd_mon _msim'_mon _msim_mon_auto : paco.
   Hint Resolve cpn8_wcompat : paco.
 
-  Definition msim_body ps pt sti_src sti_tgt fmr :=
-    @msim _ _ (@ist_with_eq _ Ist Any.t) ps pt sti_src sti_tgt fmr.
-
-  Lemma hsupd_incl P : P <1= hsupd P.
-  Proof using. ii; esplits; eauto. Qed.
-
-  Lemma hsupd_merge P r (REL : hsupd (hsupd P) r) : hsupd P r.
-  Proof using.
-    intros wf; specialize (REL wf); destruct REL as [r1 [??]].
-    hexploit Own_wand_valid; eauto.
-    intros wf1; hexploit (H wf1); intros [fmr0 [??]]; exists fmr0; esplits; eauto.
-    iIntros "R"; iPoseProof (H0 with "R") as "> R1"; iApply H2; done.
-  Qed.
-
-  Lemma hsupd_update P r r' (IN : hsupd P r) (UPD : r' ~~> r) :
-    hsupd P r'.
-  Proof using.
-    dup UPD; rewrite cmra_discrete_update in UPD; specialize (UPD (Some ε)); ss; rewrite ?right_id in UPD.
-    intros wfr'; hexploit (IN (UPD wfr')); i; des; eexists; split; eauto.
-    iIntros "H"; iPoseProof (Own_Upd with "H") as "> H"; first eauto.
-    iApply H0; done.
-  Qed.
-
-  Lemma hsupd_extends P r r' (IN : hsupd P r) (UPD : r ≼ r') :
-    hsupd P r'.
-  Proof using. eapply hsupd_update; eauto; eapply cmra_update_included; eauto. Qed.
-
-  Lemma hsupd_wf P r (IN : ✓ r → hsupd P r) :
-    hsupd P r.
-  Proof using. intros wf; hexploit (IN wf wf); i; des; clarify; esplits; eauto. Qed.
+  (* Definition msim_body ps pt sti_src sti_tgt fmr :=
+    @msim _ _ (@ist_with_eq _ Ist Any.t) ps pt sti_src sti_tgt fmr. *)
 
   Lemma _msim_flag_mon r Rs Rt RR (ps pt ps' pt' : bool) st_src st_tgt fmr
       (SIM : _msim r Rs Rt RR ps pt st_src st_tgt fmr)
@@ -419,10 +407,7 @@ Section msim.
     eapply _msim'_mon; eauto using rclo8, _msim_mon_auto; i.
   Qed.
 
-  (**
-     msim_flagC
-   **)
-
+  (** msim_flagC**)
   Variant msim_flagC
       (r : ∀ (Rs Rt : Type) (RR : retr_type Σ Rs Rt), msim_type Σ Rs Rt)
       Rs Rt RR ps1 pt1 st_src st_tgt fmr : Prop :=
@@ -465,7 +450,6 @@ Section msim.
   Lemma msim_bindC_mon r1 r2 (LEr : r1 <8= r2) : msim_bindC r1 <8= msim_bindC r2.
   Proof using. ii. destruct PR; econs; et. Qed.
 
-  (* Local Hint Resolve Own_wand_valid : core. *)
   Lemma msim_bindC_wrespectful : wrespectful8 _msim msim_bindC.
   Proof using.
     econs; eauto using msim_bindC_mon; i.
@@ -480,7 +464,7 @@ Section msim.
       try (by rr; i; esplits; eauto with paco arith);
       try (by do 2 (econs; esplits; eauto with paco arith);
               repeat rewrite <-bind_bind;
-              eauto 7 using rclo8, msim_bindC).
+              eauto 6 using rclo8, msim_bindC).
     - exploit SIMK; eauto.
       i. apply GF in x0. eapply (_msim_flag_mon _ _ _ _ _  _ ps0 pt0) in x0; try by i; clarify.
       destruct x0. eapply hsupd_update in IN; eauto.
@@ -492,10 +476,7 @@ Section msim.
   Lemma msim_bindC_spec : msim_bindC <9= gupaco8 _msim (cpn8 _msim).
   Proof using. intros. eapply wrespect8_uclo; eauto with paco. apply msim_bindC_wrespectful. Qed.
 
-  (**
-     msim_extendC
-   **)
-
+  (** msim_extendC *)
   Variant msim_extendC
     (r : ∀ Rs Rt (RR : retr_type Σ Rs Rt), msim_type Σ Rs Rt) :
     ∀ Rs Rt (RR : retr_type Σ Rs Rt), msim_type Σ Rs Rt :=
@@ -523,10 +504,7 @@ Section msim.
     eapply msim_extendC_mon, PR; eauto with paco.
   Qed.
 
-  (**
-     msim_wfC
-   **)
-
+  (** msim_wfC *)
   Variant msim_wfC (r : ∀ Rs Rt (RR : retr_type Σ Rs Rt), msim_type Σ Rs Rt):
     ∀ Rs Rt (RR : retr_type Σ Rs Rt), msim_type Σ Rs Rt :=
   | msim_wfC_intro
@@ -576,10 +554,7 @@ Section msim.
     eapply msim_updateC_mon, PR; eauto with paco.
   Qed.
 
-  (**
-     msim_frameC
-   **)
-
+  (** msim_frameC *)
   Variant msim_frameC
       (r : ∀ Rs Rt (RR : retr_type Σ Rs Rt), msim_type Σ Rs Rt) :
     ∀ Rs Rt (RR : retr_type Σ Rs Rt), msim_type Σ Rs Rt :=
@@ -628,7 +603,7 @@ Section msim.
       { iIntros "H2"; iPoseProof (H2 with "H2") as "> [H1 H2]"; iPoseProof (H4 with "H2") as "?"; iModIntro; iFrame. }
 
     - econs; eauto; intros r2 Hr2.
-      econs; intros ????; apply hsupd_merge; intros Hrv2; esplits; eauto.
+      econs; ii; apply hsupd_merge; intros Hrv2; esplits; eauto.
       revert Hr2; rewrite assoc; intros [r21 [r22 [Hr2 [Hr21 Hr22]]]]%Own_bupd_split; eauto.
       eapply (K r21); eauto.
       { rewrite Hr21 CUR; iIntros "[$ > $] //". }
@@ -820,14 +795,15 @@ Section msim.
     ∀ Rs Rt (RR : retr_type Σ Rs Rt), msim_type Σ Rs Rt :=
   | msim_nodupC_intro
       ps pt Rs Rt RR sti_src sti_tgt fmr
-      (SIM : ∀ (NODFS : List.NoDup (List.map fst fl_src))
-               (NODFT : List.NoDup (List.map fst fl_tgt))
-               (NODS : List.NoDup (List.map fst sti_src.1))
-               (NODT : List.NoDup (List.map fst sti_tgt.1)),
+      (SIM : ∀ (NODFS : map_Forall (const is_Some) (fl_src))
+               (NODFT : map_Forall (const is_Some) (fl_tgt))
+               (NODS : map_Forall (const is_Some) (sti_src.1))
+               (NODT : map_Forall (const is_Some) (sti_tgt.1)),
              r Rs Rt RR ps pt sti_src sti_tgt fmr) :
     msim_nodupC r Rs Rt RR ps pt sti_src sti_tgt fmr.
 
-  Lemma msim_nodupC_mon r1 r2 (LEr : r1 <8= r2) : msim_nodupC r1 <8= msim_nodupC r2.
+  Lemma msim_nodupC_mon r1 r2 (LEr : r1 <8= r2) :
+    msim_nodupC r1 <8= msim_nodupC r2.
   Proof using. ii. destruct PR. econs; eauto using hsupd_mon. Qed.
 
   Lemma msim_nodupC_compatible : compatible8 _msim msim_nodupC.
