theories/modules/ModTr.v
@@ -130,26 +130,26 @@ Module ModTr. Section MID.
   Definition trans_fnsem (f : Any.t → itree crisE Any.t) : Any.t → itree lmodE Any.t :=
     λ x, trans _ (f x).
 End MID. End ModTr.
-Arguments ModTr.trans {Σ T}.
+Arguments ModTr.trans {Σ} [T].
 
 Module Red. Section RED.
   Import ModTr.
   (* itree reduction lemmas *)
   Context `{Σ : GRA}.
 
-  Lemma bind {R S : Type} (s : itree crisE R) (k : R → itree crisE S) :
+  Lemma bind (R S : Type) (s : itree crisE R) (k : R → itree crisE S) :
     trans (s >>= k) = st <- trans s;; trans (k st).
   Proof using. rewrite /trans interpV_bind //. Qed.
 
-  Lemma tau {R : Type} (t : itree _ R) :
+  Lemma tau (R : Type) (t : itree _ R) :
     trans (tau;; t) = tau;; (trans t).
   Proof using. rewrite /trans interpV_tau //. Qed.
 
-  Lemma ret {R : Type} (t : R) :
+  Lemma ret (R : Type) (t : R) :
     trans (Ret t) = Ret t.
   Proof using. rewrite /trans interpV_ret //. Qed.
 
-  Lemma call {R : Type} (c : callE R) :
+  Lemma call (R : Type) (c : callE R) :
     trans (trigger c) = trigger c.
   Proof using. rewrite /trans interpV_trigger /=; grind. Qed.
 
@@ -161,33 +161,33 @@ Module Red. Section RED.
     trans (trigger (Yield tid)) = trigger (Yield tid).
   Proof using. rewrite /trans interpV_trigger /=; grind. Qed.
 
-  Lemma pg {R : Type} (i : pgE R) :
+  Lemma pg (R : Type) (i : pgE R) :
     trans (trigger i) = itreeV_itree (handle_pgE _ i).
   Proof using. rewrite /trans interpV_trigger //. Qed.
 
-  Lemma core {R : Type} (i : coreE R) :
+  Lemma core (R : Type) (i : coreE R) :
     trans (trigger i) = trigger i.
   Proof using. rewrite /trans interpV_trigger /=; grind. Qed.
 
-  Lemma triggerUB {R : Type} :
+  Lemma triggerUB (R : Type) :
     trans (triggerUB) = triggerUB (A:=R).
   Proof using.
     rewrite /trans /triggerUB interpV_bind interpV_trigger; grind.
   Qed.
 
-  Lemma triggerNB {R : Type} :
+  Lemma triggerNB (R : Type) :
     trans (triggerNB) = triggerNB (A:=R).
   Proof using.
     rewrite /trans /triggerNB interpV_bind interpV_trigger; grind.
   Qed.
 
-  Lemma unwrapU {R : Type} (i : option R) :
+  Lemma unwrapU (R : Type) (i : option R) :
     trans (@unwrapU crisE _ _ i) = unwrapU i.
   Proof using.
     rewrite /trans /unwrapU; des_ifs; s; try rewrite interpV_ret; eauto using triggerUB.
   Qed.
 
-  Lemma unwrapN {R : Type} (i : option R) :
+  Lemma unwrapN (R : Type) (i : option R) :
     trans (@unwrapN crisE _ _ i) = unwrapN i.
   Proof using.
     rewrite /trans /unwrapN; des_ifs; s; try rewrite interpV_ret; eauto using triggerNB.
@@ -205,13 +205,12 @@ Module Red. Section RED.
     trans (trigger (Guarantee P)) = itreeV_itree (handle_Guarantee P).
   Proof using. rewrite /trans interpV_trigger //. Qed.
 
-  Lemma ext {R : Type} (itr0 itr1 : itree _ R) (EQ : itr0 = itr1) :
+  Lemma ext (R : Type) (itr0 itr1 : itree _ R) (EQ : itr0 = itr1) :
     trans itr0 = trans itr1.
   Proof using. subst; et. Qed.
 
   (* TODO : Same lemmas for other interps ( not defined yet. ) *)
-
-  (* Global Program Instance rdb : red_database (mk_box (@trans)) :=
+  Global Instance rdb : red_database (mk_box (@ModTr.trans)) :=
     mk_rdb
       0
       (mk_box bind)
@@ -228,5 +227,5 @@ Module Red. Section RED.
       (mk_box unwrapN)
       (mk_box Assume)
       (mk_box Guarantee)
-      (mk_box ext). *)
+      (mk_box ext).
 End RED. End Red.
