theories/simulations/msim/ITactics.v
@@ -28,10 +28,10 @@ Ltac _istep_l :=
       iApply isim_tau_src
   | [ |- environments.envs_entails _ (isim _ _ _ _ _ _ _ _ _ (_, Ret _ >>= _) _) ] =>
       rewrite bind_ret_l
-  | [ |- environments.envs_entails _ (isim _ _ _ _ _ _ _ _ _ (_, (SB.sandbox _ _ _ (trigger (SPut _ _))) >>= _) _) ] =>
+  (* | [ |- environments.envs_entails _ (isim _ _ _ _ _ _ _ _ _ (_, (SB.sandbox _ _ _ (trigger (SPut _ _))) >>= _) _) ] =>
       iApply isim_nodup_src; iIntros (?); iApply isim_sput_src_sandbox; [s;eauto|alist_upd_simpl]
   | [ |- environments.envs_entails _ (isim _ _ _ _ _ _ _ _ _ (_, (SB.sandbox _ _ _ (trigger (SGet _))) >>= _) _) ] =>
-      iApply isim_nodup_src; iIntros (?); iApply isim_sget_src_sandbox; [s;eauto|alist_find_simpl]
+      iApply isim_nodup_src; iIntros (?); iApply isim_sget_src_sandbox; [s;eauto|alist_find_simpl] *)
   | [ |- environments.envs_entails _ (isim _ _ _ _ _ _ _ _ _ (_, trigger (Take _) >>= _) _) ] =>
       let name := fresh "_q" in
       iApply isim_take_src; iIntros (name)
@@ -69,10 +69,10 @@ Ltac _istep_r :=
       rewrite bind_ret_l
   | [ |- environments.envs_entails _ (isim _ _ _ _ _ _ _ _ _ _ (_, tau;; _)) ] =>
       iApply isim_tau_tgt
-  | [ |- environments.envs_entails _ (isim _ _ _ _ _ _ _ _ _ _ (_, (SB.sandbox _ _ _ (trigger (SPut _ _))) >>= _)) ] =>
+  (* | [ |- environments.envs_entails _ (isim _ _ _ _ _ _ _ _ _ _ (_, (SB.sandbox _ _ _ (trigger (SPut _ _))) >>= _)) ] =>
       iApply isim_nodup_tgt; iIntros (?); iApply isim_sput_tgt_sandbox; [s; eauto|alist_upd_simpl]
   | [ |- environments.envs_entails _ (isim _ _ _ _ _ _ _ _ _ _ (_, (SB.sandbox _ _ _ (trigger (SGet _))) >>= _)) ] =>
-      iApply isim_nodup_tgt; iIntros (?); iApply isim_sget_tgt_sandbox; [s; eauto|alist_find_simpl]
+      iApply isim_nodup_tgt; iIntros (?); iApply isim_sget_tgt_sandbox; [s; eauto|alist_find_simpl] *)
   | [ |- environments.envs_entails _ (isim _ _ _ _ _ _ _ _ _ _ (_, trigger (Choose _) >>= _)) ] =>
       let name := fresh "_q" in
       iApply isim_choose_tgt; iIntros (name)
@@ -168,21 +168,24 @@ Tactic Notation "iforce_r" uconstr(p) :=
 
 Ltac iforces_r := hrepeat do 1 iforce_r.
 
+(* Ltac iinline_l :=
+  norm_l with
+    do 1 iApply isim_inline_src_sandbox; [try prove_inline_cond|unfold_cris_defs].  *)
 Ltac iinline_l :=
   norm_l with
-    do 1 iApply isim_inline_src_sandbox; [try prove_inline_cond|unfold_cris_defs]. 
+    do 1 iApply isim_inline_src; [try prove_inline_cond|unfold_cris_defs]. 
 
 Ltac iinline_r :=
   norm_r with
-    do 1 iApply isim_inline_tgt_sandbox; [try prove_inline_cond|try prove_sb_cond|unfold_cris_defs].
+    do 1 iApply isim_inline_tgt; [try prove_inline_cond|try prove_sb_cond|unfold_cris_defs].
 
 Ltac icall hyps :=
-  (norm with do 1 iApply isim_call_sandbox); [try prove_sb_cond|
+  (norm with do 1 iApply isim_call); [try prove_sb_cond|
   iSplitL hyps; [try done|iIntros "% % %"; iIntrosFresh "IST"];
   move_aux].
 
 Ltac ispawn :=
-  (norm with do 1 iApply isim_spawn_sandbox); [try prove_sb_cond|].
+  (norm with do 1 iApply isim_spawn); [try prove_sb_cond|].
 
 Ltac iyield hyps :=
   (norm with do 1 iApply isim_yield);
